Prove safety for toy controller example

src/examples/controller.v
@@ -27,8 +27,8 @@ Qed.
 
 Record state := mkState {
   (* local controller state *)
-  sentCreate1: bool;
-  sentCreate2: bool;
+  sent1Create: bool;
+  sent2Create: bool;
 
   (* remote cluster state (not directly readable) *)
   obj1Exists: bool;
@@ -39,22 +39,21 @@ Record state := mkState {
 }.
 
 Instance _eta_state : Settable _ :=
-  settable! mkState<sentCreate1; sentCreate2;
+  settable! mkState<sent1Create; sent2Create;
                    obj1Exists; obj2Exists; messages>.
 
 Local Notation action := (action state).
-Local Notation predicate := (predicate state).
 Local Notation exec := (exec state).
 
 Implicit Types (s: state) (e: exec) (a: action).
 
 Definition send1_a : action :=
-  λ s s', negb s.(obj1Exists) ∧ negb s.(sentCreate1) ∧
-          s' = s <| sentCreate1 := true |> <| messages ::= (∪) {[CreateReq 1]} |>.
+  λ s s', negb s.(obj1Exists) ∧ negb s.(sent1Create) ∧
+          s' = s <| sent1Create := true |> <| messages ::= (∪) {[CreateReq 1]} |>.
 
 Definition send2_a : action :=
-  λ s s', s.(obj1Exists) ∧ s.(sentCreate1) ∧ negb s.(obj2Exists) ∧ negb s.(sentCreate2) ∧
-          s' = s <| sentCreate2 := true |> <| messages ::= (∪) {[CreateReq 2]} |>.
+  λ s s', s.(obj1Exists) ∧ s.(sent1Create) ∧ negb s.(obj2Exists) ∧ negb s.(sent2Create) ∧
+          s' = s <| sent2Create := true |> <| messages ::= (∪) {[CreateReq 2]} |>.
 
 Definition reconcile: action := λ s s', send1_a s s' ∨ send2_a s s'.
 
@@ -72,8 +71,93 @@ Definition next : action :=
   λ s s', s = s' ∨ reconcile s s' ∨ cluster s s'.
 
 Definition init s :=
-  s = {| sentCreate1 := false; sentCreate2 := false;
+  s = {| sent1Create := false; sent2Create := false;
          obj1Exists := false; obj2Exists := false;
          messages := ∅; |}.
+
+Definition safe (s: state) := s.(obj2Exists) → s.(obj1Exists).
+
+Hint Unfold init next : stm.
+Hint Unfold reconcile cluster send1_a send2_a create1 create2 : stm.
+
+Ltac stm_simp :=
+  autounfold with stm;
+  intros; intuition idtac;
+  repeat match goal with
+        | s: state |- _ => destruct s
+        | H: @eq state _ _ |- _ => inversion H; subst; clear H
+        end;
+  simpl in *;
+  intuition idtac.
+
+Ltac stm :=
+  stm_simp;
+  try solve [ intuition auto ];
+  try set_solver.
+
+Theorem messages_sent :
+  ⌜init⌝ ∧ □ ⟨next⟩ ⊢ □ ⌜λ s, (CreateReq 1 ∈ s.(messages) ↔ s.(sent1Create)) ∧
+                             (CreateReq 2 ∈ s.(messages) ↔ s.(sent2Create))⌝.
+Proof.
+  apply init_invariant.
+  - stm.
+  - stm.
+Qed.
+
+Lemma tla_pose_lemma {Σ} (p1 q1: predicate Σ) :
+  (* the lemma to introduce *)
+  (p1 ⊢ q1) →
+  ∀ (p2 q2: predicate Σ),
+  (* side condition to show precondition (to be proved by [tla_prop]) *)
+  (p2 ⊢ p1) →
+  (* the new goal *)
+  (p2 ∧ q1 ⊢ q2) →
+  (p2 ⊢ q2).
+Proof. unseal. Qed.
+
+Ltac tla_pose lem :=
+  let H := fresh "Htemp" in
+  epose proof lem as H;
+  apply (tla_pose_lemma _ _ H); clear H;
+  [ tla_prop | rewrite tla_and_assoc ].
+
+Lemma combine_preds {Σ} (next: Σ → Σ → Prop) (P: Σ → Prop) :
+  (□ ⟨ next ⟩ ∧ □ ⌜ P ⌝) == □ ⟨ λ (s s': Σ), next s s' ∧ P s ∧ P s' ⟩.
+Proof.
+  unseal.
+  intuition eauto.
+  - specialize (H k). intuition auto.
+  - specialize (H k). intuition auto.
+Qed.
+
+Theorem obj1_invariant :
+  ⌜init⌝ ∧ □ ⟨next⟩ ⊢ □ ⌜λ s, (s.(sent2Create) → s.(obj1Exists)) ∧ (s.(obj1Exists) → s.(sent1Create))⌝.
+Proof.
+  tla_pose messages_sent.
+  rewrite !combine_preds.
+  apply init_invariant.
+  - stm.
+  - stm.
+Qed.
+
+Theorem create_invariant :
+  ⌜init⌝ ∧ □ ⟨next⟩ ⊢ □ ⌜λ s, s.(obj2Exists) → s.(sent2Create) ∧ s.(sent1Create) ∧ s.(obj1Exists)⌝.
+Proof.
+  tla_pose messages_sent.
+  tla_pose obj1_invariant.
+  rewrite !combine_preds.
+  apply init_invariant.
+  - stm.
+  - stm.
+Qed.
+
+Theorem is_safe :
+  ⌜init⌝ ∧ □ ⟨next⟩ ⊢ □ ⌜safe⌝.
+Proof.
+  rewrite -> create_invariant.
+  apply always_impl_proper.
+  unseal.
+  stm.
+Qed.
 
 End example.
